rewrite_exact

FreydSSA/CFG/Fun/Subst.lean
@@ -5,18 +5,61 @@ variable {φ : Type u₁} {ν : Type u₂} {κ : Type u₃} {α : Type u₄} [Φ
   [Φc : CohInstSet φ (Ty α)]
   [DecidableEq ν] [DecidableEq κ] [DecidableEq α]
 
--- TODO: better: it's a _restriction_, i.e. L.restrict K.support = K
-def UCFG.FWfIM.toWk {L : FLCtx κ ν (Ty α)} {g : UCFG φ (Ty α) ν κ} {K : FLCtx κ ν (Ty α)}
-  : g.FWfIM L K → K.Wk L
-  | nil _ => FLCtx.Wk.refl _
-  | cons _ℓ _Γℓ _x _A dg hℓ dβ => (FLCtx.Wk.of_cons _ _ hℓ).comp dg.toWk
-  | dead _ℓ _x _A dg hℓ => dg.toWk
+def UCFG.FWfIM.to_ewk {L : FLCtx κ ν (Ty α)} {g : UCFG φ (Ty α) ν κ} {K : FLCtx κ ν (Ty α)}
+  : g.FWfIM L K → K.EWk L
+  | nil _ => FLCtx.EWk.refl _
+  | cons _ℓ _Γℓ _x _A dg hℓ dβ => (FLCtx.EWk.of_cons _ _ hℓ).trans dg.to_ewk
+  | dead _ℓ _x _A dg hℓ => dg.to_ewk
 
--- -- TODO: factor out insertion lemmas...
--- TODO: specifically restrict L' to K' to get substitution target...
--- Note we don't even need PSubstCons then!
+def UCFG.FWfIM.rewrite_exact {L' L : FLCtx κ ν (Ty α)} {g : UCFG φ (Ty α) ν κ} {K : FLCtx κ ν (Ty α)}
+  {σ : USubst φ ν}
+  (hσ : L'.PSubstCons σ L N) (dg : g.FWfIM L K) (hN : g.defs.toFinset ⊆ N)
+  (hσM : hσ.isMin)
+  (hσc : {x | x ∈ g.defs}.EqOn σ UTm.var)
+  : (g.rewrite σ).FWfIM L' (L'.restrict K.support)
+  := match dg with
+  | nil L => by
+    have h : L'.support ⊆ L.support := by rw [hσ.support_eq]
+    rw [L'.restrict_sub_support h]
+    exact nil L'
+  | cons ℓ Γℓ x A dg hℓ dβ =>
+    let dg' := dg.rewrite_exact hσ
+      (by
+        apply Finset.Subset.trans _ hN
+        simp only [defs, List.cons_append, List.toFinset_cons, List.toFinset_append]
+        apply Finset.Subset.trans (Finset.subset_union_right _ _)
+        apply Finset.subset_insert)
+      hσM (hσc.mono (λ_ => by simp only [defs]; aesop));
+    let hℓ' : ℓ ∈ (L'.restrict K.support).support := sorry;
+    let hσβ := hσ.getToFCtx ℓ (FLCtx.get _ hℓ') Γℓ x
+      sorry
+      sorry
+      sorry;
+    let ⟨Lβ', dβ', hσβ'⟩ := dβ.rewrite hσβ (by
+      apply Finset.Subset.trans _ hN
+      simp only [defs, List.cons_append, List.toFinset_cons, List.toFinset_append]
+      apply Finset.Subset.trans (Finset.subset_union_left _ _)
+      apply Finset.subset_insert
+    ) (hσc.mono (by simp only [defs, List.cons_append, List.mem_cons, List.mem_append,
+      Set.setOf_subset_setOf]; aesop));
+    have w := dg'.to_ewk.to_wk;
+    have h
+      : (L'.restrict (K.cons ℓ Γℓ).support) = (L'.restrict K.support).cons ℓ (FLCtx.get _ hℓ')
+      := sorry
+    cons ℓ _ x A (h ▸ dg') sorry (dβ'.toFWf.wkExit sorry)
+  | dead ℓ x A dg hℓ =>
+    let dg' := dg.rewrite_exact hσ
+      (by
+        apply Finset.Subset.trans _ hN
+        simp only [defs, List.cons_append, List.toFinset_cons, List.toFinset_append]
+        apply Finset.Subset.trans (Finset.subset_union_right _ _)
+        apply Finset.subset_insert)
+      hσM (hσc.mono (λ_ => by simp only [defs]; aesop));
+    dead ℓ x A dg' (hσ.not_mem_support_mpr ℓ hℓ)
+
 -- def UCFG.FWfIM.rewrite {L' L : FLCtx κ ν (Ty α)} {g : UCFG φ (Ty α) ν κ} {K : FLCtx κ ν (Ty α)}
 --   (hσ : L'.PSubstCons σ L N) (dg : g.FWfIM L K) (hN : g.defs.toFinset ⊆ N)
+--   (hσM : hσ.isMin)
 --   (hσc : {x | x ∈ g.defs}.EqOn σ UTm.var)
 --   : ΣK', (g.rewrite σ).FWfIM L' K' × K'.PSubstCons σ K N
 --   := match dg with
@@ -28,10 +71,12 @@ def UCFG.FWfIM.toWk {L : FLCtx κ ν (Ty α)} {g : UCFG φ (Ty α) ν κ} {K : F
 --       simp only [defs, List.cons_append, List.toFinset_cons, List.toFinset_append]
 --       apply Finset.Subset.trans (Finset.subset_union_right _ _)
 --       apply Finset.subset_insert)
---     (hσc.mono (λ_ => by simp only [defs]; aesop))
---   let ⟨Γℓ', hK'⟩ := hσ'.consSrc;
---   let hσβ := hσ.getToFCtx ℓ Γℓ' Γℓ x sorry sorry sorry;
---   -- TODO: rewrite rather than subst...
+--     hσM (hσc.mono (λ_ => by simp only [defs]; aesop))
+--   let hℓ := hσ'.consSrc;
+--   let hσβ := hσ.getToFCtx ℓ (K'.get _ hℓ) Γℓ x
+--     sorry
+--     sorry
+--     sorry;
 --   let ⟨Lβ', dβ', hσβ'⟩ := dβ.rewrite hσβ (by
 --     apply Finset.Subset.trans _ hN
 --     simp only [defs, List.cons_append, List.toFinset_cons, List.toFinset_append]
@@ -44,7 +89,7 @@ def UCFG.FWfIM.toWk {L : FLCtx κ ν (Ty α)} {g : UCFG φ (Ty α) ν κ} {K : F
 --   ⟨
 --     K'.erase ℓ,
 --     cons ℓ _ x A (hK' ▸ dg') (by simp [FLCtx.erase]) (dβ'.toFWf.wkExit sorry),
---     sorry
+--     hσ'.erase' ℓ sorry rfl
 --   ⟩
 --   | dead ℓ x A dg hℓ =>
 --     let ⟨K', dg', hσ'⟩ := dg.rewrite hσ
@@ -53,7 +98,7 @@ def UCFG.FWfIM.toWk {L : FLCtx κ ν (Ty α)} {g : UCFG φ (Ty α) ν κ} {K : F
 --         simp only [defs, List.cons_append, List.toFinset_cons, List.toFinset_append]
 --         apply Finset.Subset.trans (Finset.subset_union_right _ _)
 --         apply Finset.subset_insert)
---       (hσc.mono (λ_ => by simp only [defs]; aesop));
+--       hσM (hσc.mono (λ_ => by simp only [defs]; aesop));
 --     ⟨K', dead ℓ x A dg' (hσ.not_mem_support_mpr ℓ hℓ), hσ'⟩
 
 -- def UCFG.FWfI.subst {L' L : FLCtx κ ν (Ty α)} {g : UCFG φ (Ty α) ν κ} {K : FLCtx κ ν (Ty α)}
